strcmp_proofs.v
@@ -98,6 +98,7 @@ Definition strcmp_esp_invset esp0 :=
    anywhere an invariant exists (e.g., at the post-condition), it is true. *)
 Theorem strcmp_preserves_esp:
   forall s esp0 mem n s' x'
+         (MDL0: models x86typctx s)
          (ESP0: s R_ESP = Ⓓ esp0) (MEM0: s V_MEM32 = Ⓜ mem)
          (RET: strcmp_i386 s (mem Ⓓ[esp0]) = None)
          (XP0: exec_prog fh strcmp_i386 0 s n s' x'),
@@ -123,10 +124,12 @@ Proof.
      can get the value of MEM from MEM0 using our previously proved strlen_preserves_memory
      theorem. *)
   intros.
+  assert (MDL: models x86typctx s1).
+    eapply preservation_exec_prog. exact MDL0. apply strcmp_welltyped. exact XP.
   assert (MEM: s1 V_MEM32 = Ⓜ mem).
     rewrite <- MEM0. eapply strlen_preserves_memory. exact XP.
   rewrite (strcmp_nwc s1) in RET.
-  clear s MEM0 XP0 ESP0 XP.
+  clear s MDL0 MEM0 XP0 ESP0 XP.
 
   (* We are now ready to break the goal down into one case for each invariant-point.
      The destruct_inv tactic finds all the invariants defined by the invariant-set
@@ -220,7 +223,7 @@ Proof.
     rewrite <- MEM0. eapply strlen_preserves_memory. exact XP.
   assert (WTM := x86_wtm MDL MEM). simpl in WTM.
   rewrite (strcmp_nwc s1) in RET.
-  assert (ESP := strcmp_preserves_esp _ _ _ _ _ (Exit a1) ESP0 MEM0 RET XP).
+  assert (ESP := strcmp_preserves_esp _ _ _ _ _ (Exit a1) MDL0 ESP0 MEM0 RET XP).
   clear s MDL0 MEM0 ESP0 XP XP0.
 
   (* Break the proof into cases, one for each invariant-point. *)
